StrataTest/Languages/GOTO/CFGToCProverGOTO.lean
@@ -32,7 +32,8 @@ private abbrev LExprTP : Imperative.PureExpr :=
      TyEnv := @Lambda.TEnv TestParams.IDMeta,
      TyContext := @Lambda.LContext TestParams,
      EqIdent := inferInstanceAs (DecidableEq TestParams.Identifier)
-     Factory := Unit }
+     Factory := Unit,
+     eval := fun _f _σ e => some e }
 
 private def lookupType (T : LExprTP.TyEnv) (i : LExprTP.Ident) : Except Format CProverGOTO.Ty :=
   match T.context.types.find? i with
